tests/deftype_tests.rs
@@ -1,0 +1,142 @@
+use lisp_rlm::EvalState;
+use lisp_rlm::*;
+
+fn run_all(code: &str) -> Result<String, String> {
+    let exprs = parse_all(code)?;
+    let mut env = Env::new();
+    let mut state = EvalState::new();
+    let mut result = LispVal::Nil;
+    for expr in &exprs {
+        result = lisp_rlm::program::run_program(&[expr.clone()], &mut env, &mut state)?;
+    }
+    Ok(result.to_string())
+}
+
+fn eval(code: &str) -> String {
+    run_all(code).unwrap_or_else(|e| format!("ERROR: {}", e))
+}
+
+#[test]
+fn test_deftype_basic() {
+    assert_eq!(eval(r#"(deftype (Option a) (Some a) None) (Some 42)"#), "(Option::0 42)");
+}
+
+#[test]
+fn test_deftype_nullary() {
+    assert_eq!(eval(r#"(deftype (Option a) (Some a) None) None"#), "#<Option::1>");
+}
+
+#[test]
+fn test_deftype_multi_field() {
+    assert_eq!(eval(r#"(deftype Result (Ok val) (Err msg)) (Ok 42)"#), "(Result::0 42)");
+}
+
+#[test]
+fn test_deftype_tag_test_positive() {
+    assert_eq!(eval(r#"
+(deftype (Option a) (Some a) None)
+(let ((x (Some 42))) (tag-test x "Option::0"))
+"#), "true");
+}
+
+#[test]
+fn test_deftype_tag_test_negative() {
+    assert_eq!(eval(r#"
+(deftype (Option a) (Some a) None)
+(let ((x (Some 42))) (tag-test x "Option::1"))
+"#), "false");
+}
+
+#[test]
+fn test_deftype_get_field() {
+    assert_eq!(eval(r#"
+(deftype (Option a) (Some a) None)
+(let ((x (Some 42))) (get-field x 0))
+"#), "42");
+}
+
+#[test]
+fn test_deftype_pattern_match_some() {
+    assert_eq!(eval(r#"
+(deftype (Option a) (Some a) None)
+(define (unwrap-or opt default)
+  (if (tag-test opt "Option::0")
+    (get-field opt 0)
+    default))
+(unwrap-or (Some 99) 0)
+"#), "99");
+}
+
+#[test]
+fn test_deftype_pattern_match_none() {
+    assert_eq!(eval(r#"
+(deftype (Option a) (Some a) None)
+(define (unwrap-or opt default)
+  (if (tag-test opt "Option::0")
+    (get-field opt 0)
+    default))
+(unwrap-or None 7)
+"#), "7");
+}
+
+#[test]
+fn test_deftype_nested() {
+    assert_eq!(eval(r#"
+(deftype (Option a) (Some a) None)
+(deftype Result (Ok val) (Err msg))
+(Ok (Some "hello"))
+"#), "(Result::0 (Option::0 \"hello\"))");
+}
+
+#[test]
+fn test_deftype_in_function() {
+    assert_eq!(eval(r#"
+(deftype (Option a) (Some a) None)
+(define (wrap x) (Some x))
+(wrap 42)
+"#), "(Option::0 42)");
+}
+
+#[test]
+fn test_deftype_equality() {
+    assert_eq!(eval(r#"
+(deftype (Option a) (Some a) None)
+(= (Some 1) (Some 1))
+"#), "true");
+}
+
+#[test]
+fn test_deftype_higher_order_map() {
+    assert_eq!(eval(r#"
+(deftype (Option a) (Some a) None)
+(map (fn (x) (Some (* x 2))) (list 1 2 3))
+"#), "((Option::0 2) (Option::0 4) (Option::0 6))");
+}
+
+#[test]
+fn test_deftype_err_variant() {
+    assert_eq!(eval(r#"
+(deftype Result (Ok val) (Err msg))
+(Err "something went wrong")
+"#), "(Result::1 \"something went wrong\")");
+}
+
+#[test]
+fn test_deftype_two_fields() {
+    assert_eq!(eval(r#"
+(deftype Pair (MkPair fst snd))
+(MkPair 10 20)
+"#), "(Pair::0 10 20)");
+}
+
+#[test]
+fn test_deftype_recursive_pattern() {
+    assert_eq!(eval(r#"
+(deftype (Option a) (Some a) None)
+(define (map-opt f opt)
+  (if (tag-test opt "Option::0")
+    (Some (f (get-field opt 0)))
+    None))
+(map-opt (fn (x) (* x 10)) (Some 5))
+"#), "(Option::0 50)");
+}
